\documentclass[12pt]{extarticle} 
\usepackage[T2A]{fontenc} 
\usepackage[cp1251]{inputenc}
\usepackage[russian]{babel}
\usepackage{mathtext}
\usepackage{graphicx}
\usepackage{graphics}
\usepackage{caption}
\usepackage{subcaption}
\usepackage{amsmath}
\usepackage{amsthm}
\usepackage{lscape}
\usepackage{makecell}
\usepackage{multirow}
\usepackage{ulem}
\usepackage{indentfirst}
\usepackage{enumerate}
\usepackage{amssymb}
\usepackage{setspace}
\usepackage[left=3cm, right=2cm, top=2cm, bottom=2cm]{geometry}

\parindent=1cm
\pagestyle{plain}
\onehalfspacing

\begin{document}

\begin{equation}
	\dot u = u'' + \gamma u - u^3,	
\end{equation}
\begin{equation}
	u'(0, t) \, = 0, \qquad u'(1, t) \, = \alpha\,u(x_0, t),
\end{equation}
$ \alpha, \gamma \in \mathbb{R}, \; x_0 \in [0, 1). $

\begin{equation}
	\dot u = u'' + \gamma u,	
\end{equation}
\begin{equation}	
	u'(0, t) \, = 0, \qquad u'(1, t) \, = \alpha\,u(x_0, t).
\end{equation}
$ u(x, t) = e^{\lambda t} \, v(x). $

\begin{equation}
	v'' + (\gamma - \lambda)v = 0,	
\end{equation}
\begin{equation}	
	v'(0) \, = 0, \qquad v'(1) \, = \alpha\,v(x_0).
\end{equation}
$ \mu = \sqrt{-\gamma + \lambda}, \; v(x) = c \, \mbox{ch}  \mu x, \; c \in \mathbb{R}. $

$$ \mu \, \mbox{sh} \mu \, = \, \alpha \mbox{ch} \mu x_0 , $$
\begin{equation}
	\alpha_{cr} = \frac{\mu \, \mbox{sh} \mu}{\mbox{ch} \mu x_0}.
\end{equation}

\begin{equation} 
	\dot{u}_j =  n^2(u_{j+1} - 2u_j + u_{j-1}) + \gamma u_j - u_j^3, \quad j = \overline{1, n}. 
\end{equation}
\begin{gather}	
	u_0 = u_1, \quad u_{n+1} = u_n + \frac{\alpha_c}{n}\:u_1.
\end{gather}

\begin{equation}
	u = \sqrt{\varepsilon}u_0 + \varepsilon u_1 + \varepsilon^{\frac{3}{2}} u_2 + O(\varepsilon^2).
\end{equation}

\begin{equation}
	v'' + \gamma v = 0,
\end{equation}
\begin{equation}
	v'(0) = 0, \quad v'(1) = \alpha_{cr}\,v(x_0).
\end{equation}

\begin{equation}
	\frac{\partial u_0}{\partial s} + \dot{u}_2 = u''_2 + \gamma u_2 - u_0^3,
\end{equation}
\begin{equation}
u_2'(0, t) = 0, \quad u_2'(1, t) = \alpha_{cr}\,u_2(x_0, t) + u_0(x_0, t).
\end{equation}
$ s = \varepsilon t. $

\newpage

$ \lambda = 0: \mu = \sqrt{-\gamma}, \; \alpha_{cr} = \alpha_d, \; \varepsilon=\alpha-\alpha_d. $

\begin{equation}
	u_0 = \rho(s) \mbox{ch} \mu x.
\end{equation}
\begin{equation}
	\rho' = \phi \rho + d \rho^3,
\end{equation}
$$ \phi = \frac{ 2 \mu \mbox{ch} \mu x_0 }{ \mu \mbox{ch} \mu +\mbox{sh} \mu - \alpha_d x_0 \mbox{sh} \mu x_0 }, $$
$$ d = \frac{ -3\gamma \mbox{sh} 3\mu - 12 \mbox{sh} \mu - 12 \mu \mbox{ch} \mu - \alpha_d \mu \mbox{ch} 3\mu x_0 + 12 \alpha_d x_0 \mbox{sh} \mu x_0 }{ 16( \mbox{sh} \mu + \mu \mbox{ch} \mu - \alpha_d x_0 \mbox{sh} \mu x_0 ) }. $$

$ \lambda = i \omega: \mu = \sqrt{-\gamma + i \omega}, \; \alpha_{cr} = \alpha_c, \; \varepsilon=\alpha_c-\alpha. $

\begin{equation}
	u_0 = z(s) e^{i \omega t} \mbox{ch} \mu x + \overline{z(s)} e^{-i \omega t} \overline{\mbox{ch} \mu x}.
\end{equation}
\begin{equation}
	z' = \phi z + d z |z|^2.
\end{equation}
$$ \phi = \frac{ 2 \mu \mbox{ch} \mu x_0 }{ \mu \mbox{ch} \mu +\mbox{sh} \mu - \alpha_c x_0 \mbox{sh} \mu x_0 }, $$
$$ d = \frac{ 3 \mu ( G(\mu + 2\,\mbox{Re}\mu) + G(\mu + 2i\,\mbox{Im}\mu) + 2G(\overline{\mu}) ) }{ 2 ( \mu \mbox{ch} \mu +\mbox{sh} \mu - \alpha_c x_0 \mbox{sh} \mu x_0 ) }, $$
$$ G(y) = \frac{ \alpha_c - y\,\mbox{sh} y }{ y^2 + \gamma - i\omega }. $$

\end{document}